Improve notations for atomic triples.

theories/zoo/iris/program_logic/atomic.v
@@ -150,255 +150,20 @@ Section atomic_update.
   Qed.
 End atomic_update.
 
-Section atomic_wp.
-  Context `{iris_GS : !IrisG Λ Σ} {TA TB : tele}.
-
-  Implicit Types α : TA → iProp Σ.
-  Implicit Types β Ψ : TA → TB → iProp Σ.
-  Implicit Types f : TA → TB → val Λ.
-
-  Definition atomic_wp e E α β Ψ f : iProp Σ :=
-    ∀ Φ,
-    atomic_update (⊤ ∖ E) ∅ α β (λ.. x y, Ψ x y -∗ Φ (f x y)) -∗
-    WP e {{ Φ }}.
-  #[global] Arguments atomic_wp e%_E E (α β Ψ f)%_I : assert.
-
-  #[global] Instance atomic_wp_ne e E n :
-    Proper (
-      pointwise_relation TA (≡{n}≡) ==>
-      pointwise_relation TA (pointwise_relation TB (≡{n}≡)) ==>
-      pointwise_relation TA (pointwise_relation TB (≡{n}≡)) ==>
-      pointwise_relation TA (pointwise_relation TB (=)) ==>
-      (≡{n}≡)
-    ) (atomic_wp e E).
-  Proof.
-    intros α1 α2 Hα β1 β2 Hβ Ψ1 Ψ2 HΨ f1 f2 Hf. rewrite /atomic_wp.
-    f_equiv. intros Φ. do 2 f_equiv; [done.. |]. intros x y.
-    rewrite !tele_app_bind. solve_proper.
-  Qed.
-  #[global] Instance atomic_wp_proper e E :
-    Proper (
-      pointwise_relation TA (≡) ==>
-      pointwise_relation TA (pointwise_relation TB (≡)) ==>
-      pointwise_relation TA (pointwise_relation TB (≡)) ==>
-      pointwise_relation TA (pointwise_relation TB (=)) ==>
-      (≡)
-    ) (atomic_wp e E).
-  Proof.
-    intros α1 α2 Hα β1 β2 Hβ Ψ1 Ψ2 HΨ f1 f2 Hf. rewrite /atomic_wp.
-    f_equiv. intros Φ. do 2 f_equiv; [done.. |]. intros x y.
-    rewrite !tele_app_bind. f_equiv; first solve_proper. f_equiv. apply Hf.
-  Qed.
-
-  Lemma atomic_wp_mono e E α β Ψ1 Ψ2 f :
-    (∀.. x y, Ψ1 x y -∗ Ψ2 x y) -∗
-    atomic_wp e E α β Ψ1 f -∗
-    atomic_wp e E α β Ψ2 f.
-  Proof.
-    iIntros "HΨ H %Φ HΦ".
-    iApply "H".
-    iApply (atomic_update_wand with "HΦ"). iIntros "%x %y HΨ2". rewrite !tele_app_bind. iIntros "HΨ1".
-    iApply "HΨ2".
-    iApply "HΨ".
-    iSteps.
-  Qed.
-  Lemma atomic_wp_wand e E α β Ψ1 Ψ2 f :
-    atomic_wp e E α β Ψ1 f -∗
-    (∀.. x y, Ψ1 x y -∗ Ψ2 x y) -∗
-    atomic_wp e E α β Ψ2 f.
-  Proof.
-    iIntros "H HΨ".
-    iApply (atomic_wp_mono with "HΨ H").
-  Qed.
-
-  Lemma atomic_wp_frame_l R e E α β Ψ f :
-    R ∗ atomic_wp e E α β Ψ f ⊢
-    atomic_wp e E α β (λ x y, R ∗ Ψ x y) f.
-  Proof.
-    iIntros "(HR & H)".
-    iApply (atomic_wp_wand with "H").
-    iSteps.
-  Qed.
-  Lemma atomic_wp_frame_r R e E α β Ψ f :
-    atomic_wp e E α β Ψ f ∗ R ⊢
-    atomic_wp e E α β (λ x y, Ψ x y ∗ R) f.
-  Proof.
-    iIntros "(H & HR)".
-    iApply (atomic_wp_wand with "H").
-    iSteps.
-  Qed.
-
-  Lemma atomic_wp_mask_weaken E1 E2 e α β Ψ f :
-    E1 ⊆ E2 →
-    atomic_wp e E1 α β Ψ f ⊢
-    atomic_wp e E2 α β Ψ f.
-  Proof.
-    rewrite /atomic_wp => HE.
-    iIntros "H %Φ HΦ".
-    iDestruct (atomic_update_mask_weaken _ (⊤ ∖ E1) with "HΦ") as "HΦ"; first solve_ndisj.
-    iSteps.
-  Qed.
-
-  #[global] Instance frame_atomic_wp p R e E α β Ψ1 Ψ2 f :
-    (∀ x y, Frame p R (Ψ1 x y) (Ψ2 x y)) →
-    Frame p R (atomic_wp e E α β (λ.. x y, Ψ1 x y) f) (atomic_wp e E α β (λ.. x y, Ψ2 x y) f).
-  Proof.
-    rewrite /Frame atomic_wp_frame_l => HΨ.
-    iApply atomic_wp_mono. iIntros "%x %y". rewrite !tele_app_bind.
-    iApply HΨ.
-  Qed.
-
-  #[global] Instance is_except_0_atomic_wp e E α β Ψ f :
-    IsExcept0 (atomic_wp e E α β Ψ f).
-  Proof.
-    rewrite /IsExcept0. iIntros ">$".
-  Qed.
-End atomic_wp.
-
-Notation "'AWP' '<<' ∀∀ x1 .. xn , α '>>' e @ E '<<' ∃∃ y1 .. yn , β | 'RET' v ; Q '>>'" := (
-  atomic_wp
-    (TA := TeleS (λ x1, .. (TeleS (λ xn, TeleO)) .. ))
-    (TB := TeleS (λ y1, .. (TeleS (λ yn, TeleO)) .. ))
-    e%E
-    E
-    (tele_app $ λ x1, .. (λ xn, α%I) ..)
-    (tele_app $ λ x1, .. (λ xn, tele_app (λ y1, .. (λ yn, β%I) .. )) .. )
-    (tele_app $ λ x1, .. (λ xn, tele_app (λ y1, .. (λ yn, Q%I) .. )) .. )
-    (tele_app $ λ x1, .. (λ xn, tele_app (λ y1, .. (λ yn, v%V) .. )) .. )
-)(at level 20,
-  α, e, E, β, v, Q at level 200,
-  x1 binder,
-  xn binder,
-  y1 binder,
-  yn binder,
-  format "'[hv' '[' 'AWP'  '<<'  ∀∀  x1  ..  xn ,  '/  ' '[' α ']'  '/' '>>' ']'  '/  ' e  '/  ' @  E  '/' '[' '<<'  ∃∃ y1  ..  yn ,  '/  ' '[' β  |  '/' RET v ;  Q ']'  '/' '>>' ']' ']'"
-) : bi_scope.
-Notation "'AWP' '<<' α '>>' e @ E '<<' ∃∃ y1 .. yn , β | 'RET' v ; Q '>>'" := (
-  atomic_wp
-    (TA := TeleO)
-    (TB := TeleS (λ y1, .. (TeleS (λ yn, TeleO)) .. ))
-    e%E
-    E
-    (tele_app α%I)
-    (tele_app $ tele_app (λ y1, .. (λ yn, β%I) .. ))
-    (tele_app $ tele_app (λ y1, .. (λ yn, Q%I) .. ))
-    (tele_app $ tele_app (λ y1, .. (λ yn, v%V) .. ))
-)(at level 20,
-  α, e, E, β, v, Q at level 200,
-  y1 binder,
-  yn binder,
-  format "'[hv' '[' 'AWP'  '<<'  '/  ' '[' α ']'  '/' '>>' ']'  '/  ' e  '/  ' @  E  '/' '[' '<<'  ∃∃ y1  ..  yn ,  '/  ' '[' β  |  '/' RET v ;  Q ']'  '/' '>>' ']' ']'"
-) : bi_scope.
-Notation "'AWP' '<<' ∀∀ x1 .. xn , α '>>' e @ E '<<' β | 'RET' v ; Q '>>'" := (
-  atomic_wp
-    (TA := TeleS (λ x1, .. (TeleS (λ xn, TeleO)) .. ))
-    (TB := TeleO)
-    e%E
-    E
-    (tele_app $ λ x1, .. (λ xn, α%I) ..)
-    (tele_app $ λ x1, .. (λ xn, tele_app β%I) .. )
-    (tele_app $ λ x1, .. (λ xn, tele_app Q%I) .. )
-    (tele_app $ λ x1, .. (λ xn, tele_app v%V) .. )
-)(at level 20,
-  α, e, E, β, v, Q at level 200,
-  x1 binder,
-  xn binder,
-  format "'[hv' '[' 'AWP'  '<<'  ∀∀  x1  ..  xn ,  '/  ' '[' α ']'  '/' '>>' ']'  '/  ' e  '/  ' @  E  '/' '[' '<<'  '/  ' '[' β  |  '/' RET v ;  Q ']'  '/' '>>' ']' ']'"
-) : bi_scope.
-Notation "'AWP' '<<' α '>>' e @ E '<<' β | 'RET' v ; Q '>>'" := (
-  atomic_wp
-    (TA := TeleO)
-    (TB := TeleO)
-    e%E
-    E
-    (tele_app α%I)
-    (tele_app $ tele_app β%I)
-    (tele_app $ tele_app Q%I)
-    (tele_app $ tele_app v%V)
-)(at level 20,
-  α, e, E, β, v, Q at level 200,
-  format "'[hv' '[' 'AWP'  '<<'  '/  ' '[' α ']'  '/' '>>' ']'  '/  ' e  '/  ' @  E  '/' '[' '<<'  '/  ' '[' β  |  '/' RET v ;  Q ']'  '/' '>>' ']' ']'"
-) : bi_scope.
-Notation "'AWP' '<<' ∀∀ x1 .. xn , α '>>' e '<<' ∃∃ y1 .. yn , β | 'RET' v ; Q '>>'" := (
-  atomic_wp
-    (TA := TeleS (λ x1, .. (TeleS (λ xn, TeleO)) .. ))
-    (TB := TeleS (λ y1, .. (TeleS (λ yn, TeleO)) .. ))
-    e%E
-    ∅
-    (tele_app $ λ x1, .. (λ xn, α%I) ..)
-    (tele_app $ λ x1, .. (λ xn, tele_app (λ y1, .. (λ yn, β%I) .. )) .. )
-    (tele_app $ λ x1, .. (λ xn, tele_app (λ y1, .. (λ yn, Q%I) .. )) .. )
-    (tele_app $ λ x1, .. (λ xn, tele_app (λ y1, .. (λ yn, v%V) .. )) .. )
-)(at level 20,
-  α, e, β, v, Q at level 200,
-  x1 binder,
-  xn binder,
-  y1 binder,
-  yn binder,
-  format "'[hv' '[' 'AWP'  '<<'  ∀∀  x1  ..  xn ,  '/  ' '[' α ']'  '/' '>>' ']'  '/  ' e  '/' '[' '<<'  ∃∃ y1  ..  yn ,  '/  ' '[' β  |  '/' RET v ;  Q ']'  '/' '>>' ']' ']'"
-) : bi_scope.
-Notation "'AWP' '<<' α '>>' e '<<' ∃∃ y1 .. yn , β | 'RET' v ; Q '>>'" := (
-  atomic_wp
-    (TA := TeleO)
-    (TB := TeleS (λ y1, .. (TeleS (λ yn, TeleO)) .. ))
-    e%E
-    ∅
-    (tele_app α%I)
-    (tele_app $ tele_app (λ y1, .. (λ yn, β%I) .. ))
-    (tele_app $ tele_app (λ y1, .. (λ yn, Q%I) .. ))
-    (tele_app $ tele_app (λ y1, .. (λ yn, v%V) .. ))
-)(at level 20,
-  α, e, β, v, Q at level 200,
-  y1 binder,
-  yn binder,
-  format "'[hv' '[' 'AWP'  '<<'  '/  ' '[' α ']'  '/' '>>' ']'  '/  ' e  '/' '[' '<<'  ∃∃ y1  ..  yn ,  '/  ' '[' β  |  '/' RET v ;  Q ']'  '/' '>>' ']' ']'"
-) : bi_scope.
-Notation "'AWP' '<<' ∀∀ x1 .. xn , α '>>' e '<<' β | 'RET' v ; Q '>>'" := (
-  atomic_wp
-    (TA := TeleS (λ x1, .. (TeleS (λ xn, TeleO)) .. ))
-    (TB := TeleO)
-    e%E
-    ∅
-    (tele_app $ λ x1, .. (λ xn, α%I) ..)
-    (tele_app $ λ x1, .. (λ xn, tele_app β%I) .. )
-    (tele_app $ λ x1, .. (λ xn, tele_app Q%I) .. )
-    (tele_app $ λ x1, .. (λ xn, tele_app v%V) .. )
-)(at level 20,
-  α, e, β, v, Q at level 200,
-  x1 binder,
-  xn binder,
-  format "'[hv' '[' 'AWP'  '<<'  ∀∀  x1  ..  xn ,  '/  ' '[' α ']'  '/' '>>' ']'  '/  ' e  '/' '[' '<<'  '/  ' '[' β  |  '/' RET v ;  Q ']'  '/' '>>' ']' ']'"
-) : bi_scope.
-Notation "'AWP' '<<' α '>>' e '<<' β | 'RET' v ; Q '>>'" := (
-  atomic_wp
-    (TA := TeleO)
-    (TB := TeleO)
-    e%E
-    ∅
-    (tele_app α%I)
-    (tele_app $ tele_app β%I)
-    (tele_app $ tele_app Q%I)
-    (tele_app $ tele_app v%V)
-)(at level 20,
-  α, e, β, v, Q at level 200,
-  format "'[hv' '[' 'AWP'  '<<'  '/  ' '[' α ']'  '/' '>>' ']'  '/  ' e  '/' '[' '<<'  '/  ' '[' β  |  '/' RET v ;  Q ']'  '/' '>>' ']' ']'"
-) : bi_scope.
-
 Section atomic_triple.
-  Context `{iris_G : !IrisG Λ Σ} {TA TB : tele}.
+  Context `{iris_G : !IrisG Λ Σ} {TA TB TP : tele}.
 
   Implicit Types P : iProp Σ.
   Implicit Types α : TA → iProp Σ.
-  Implicit Types β Ψ : TA → TB → iProp Σ.
-  Implicit Types f : TA → TB → val Λ.
+  Implicit Types β : TA → TB → iProp Σ.
+  Implicit Types Ψ : TA → TB → TP → iProp Σ.
+  Implicit Types f : TA → TB → TP → val Λ.
 
   Definition atomic_triple e E P α β Ψ f : iProp Σ :=
-    □ (
-      ∀ Φ,
-      P -∗
-      atomic_update (⊤ ∖ E) ∅ α β (λ.. x y, Ψ x y -∗ Φ (f x y)) -∗
-      WP e {{ Φ }}
-    ).
+    ∀ Φ,
+    P -∗
+    atomic_update (⊤ ∖ E) ∅ α β (λ.. x y, ∀.. z, Ψ x y z -∗ Φ (f x y z)) -∗
+    WP e {{ Φ }}.
   #[global] Arguments atomic_triple e%_E E (P α β Ψ f)%_I : assert.
 
   #[global] Instance atomic_triple_ne e E n :
@@ -406,68 +171,75 @@ Section atomic_triple.
       (≡{n}≡) ==>
       pointwise_relation TA (≡{n}≡) ==>
       pointwise_relation TA (pointwise_relation TB (≡{n}≡)) ==>
-      pointwise_relation TA (pointwise_relation TB (≡{n}≡)) ==>
-      pointwise_relation TA (pointwise_relation TB (=)) ==>
+      pointwise_relation TA (pointwise_relation TB (pointwise_relation TP (≡{n}≡))) ==>
+      pointwise_relation TA (pointwise_relation TB (pointwise_relation TP (=))) ==>
       (≡{n}≡)
     ) (atomic_triple e E).
   Proof.
-    intros P1 P2 HP α1 α2 Hα β1 β2 Hβ Ψ1 Ψ2 HΨ f1 f2 Hf. rewrite /atomic_triple.
-    do 2 f_equiv. intros Φ. f_equiv; first done. do 2 f_equiv; [done.. |]. intros x y.
-    rewrite !tele_app_bind. solve_proper.
+    rewrite /atomic_triple => P1 P2 HP α1 α2 Hα β1 β2 Hβ Ψ1 Ψ2 HΨ f1 f2 Hf.
+    do 3 f_equiv; first done.
+    do 2 f_equiv; [done.. |].
+    intros x y. rewrite !tele_app_bind.
+    do 3 f_equiv; first apply HΨ.
+    f_equiv. apply Hf.
   Qed.
   #[global] Instance atomic_triple_proper e E :
     Proper (
       (≡) ==>
       pointwise_relation TA (≡) ==>
       pointwise_relation TA (pointwise_relation TB (≡)) ==>
-      pointwise_relation TA (pointwise_relation TB (≡)) ==>
-      pointwise_relation TA (pointwise_relation TB (=)) ==>
+      pointwise_relation TA (pointwise_relation TB (pointwise_relation TP (≡))) ==>
+      pointwise_relation TA (pointwise_relation TB (pointwise_relation TP (=))) ==>
       (≡)
     ) (atomic_triple e E).
   Proof.
-    intros P1 P2 HP α1 α2 Hα β1 β2 Hβ Ψ1 Ψ2 HΨ f1 f2 Hf. rewrite /atomic_triple.
-    do 2 f_equiv. intros Φ. f_equiv; first done. do 2 f_equiv; [done.. |]. intros x y.
-    rewrite !tele_app_bind. f_equiv; first solve_proper. f_equiv.
-    rewrite leibniz_equiv_iff. solve_proper.
+    rewrite /atomic_triple => P1 P2 HP α1 α2 Hα β1 β2 Hβ Ψ1 Ψ2 HΨ f1 f2 Hf.
+    do 3 f_equiv; first done.
+    do 2 f_equiv; [done.. |].
+    intros x y. rewrite !tele_app_bind.
+    do 3 f_equiv; first apply HΨ.
+    f_equiv. apply Hf.
   Qed.
 
   Lemma atomic_triple_mono e E P α β Ψ1 Ψ2 f :
-    □ (∀.. x y, Ψ1 x y -∗ Ψ2 x y) -∗
+    (∀.. x y z, Ψ1 x y z -∗ Ψ2 x y z) -∗
     atomic_triple e E P α β Ψ1 f -∗
     atomic_triple e E P α β Ψ2 f.
   Proof.
-    iIntros "#HΨ #H !> %Φ HP HΦ".
+    iIntros "HΨ H %Φ HP HΦ".
     iApply ("H" with "HP").
-    iApply (atomic_update_wand with "HΦ"). iIntros "%x %y HΨ2". rewrite !tele_app_bind. iIntros "HΨ1".
+    iApply (atomic_update_wand with "HΦ"). iIntros "%x %y HΨ2". rewrite !tele_app_bind. iIntros "%z HΨ1".
     iApply "HΨ2".
     iApply "HΨ".
     iSteps.
   Qed.
   Lemma atomic_triple_wand e E P α β Ψ1 Ψ2 f :
     atomic_triple e E P α β Ψ1 f -∗
-    □ (∀.. x y, Ψ1 x y -∗ Ψ2 x y) -∗
+    (∀.. x y z, Ψ1 x y z -∗ Ψ2 x y z) -∗
     atomic_triple e E P α β Ψ2 f.
   Proof.
-    iIntros "#H #HΨ".
+    iIntros "H HΨ".
     iApply (atomic_triple_mono with "HΨ H").
   Qed.
 
   Lemma atomic_triple_frame_l R e E P α β Ψ f :
     atomic_triple e E P α β Ψ f ⊢
-    atomic_triple e E (R ∗ P) α β (λ x y, R ∗ Ψ x y) f.
+    atomic_triple e E (R ∗ P) α β (λ x y z, R ∗ Ψ x y z) f.
   Proof.
-    iIntros "#H !> %Φ (HR & HP) HΦ".
+    iIntros "H %Φ (HR & HP) HΦ".
     iApply ("H" with "HP").
-    iApply (atomic_update_wand with "HΦ"). iIntros "%x %y HΦ". rewrite !tele_app_bind.
+    iApply (atomic_update_wand with "HΦ"). iIntros "%x %y HΦ". rewrite !tele_app_bind. iIntros "%z HΨ".
+    iApply "HΦ".
     iSteps.
   Qed.
   Lemma atomic_triple_frame_r R e E P α β Ψ f :
     atomic_triple e E P α β Ψ f ⊢
-    atomic_triple e E (P ∗ R) α β (λ x y, Ψ x y ∗ R) f.
+    atomic_triple e E (P ∗ R) α β (λ x y z, Ψ x y z ∗ R) f.
   Proof.
-    iIntros "#H !> %Φ (HP & HR) HΦ".
+    iIntros "H %Φ (HP & HR) HΦ".
     iApply ("H" with "HP").
-    iApply (atomic_update_wand with "HΦ"). iIntros "%x %y HΦ". rewrite !tele_app_bind.
+    iApply (atomic_update_wand with "HΦ"). iIntros "%x %y HΦ". rewrite !tele_app_bind. iIntros "%z HΨ".
+    iApply "HΦ".
     iSteps.
   Qed.
 
@@ -477,34 +249,56 @@ Section atomic_triple.
     atomic_triple e E2 P α β Ψ f.
   Proof.
     rewrite /atomic_triple => HE.
-    iIntros "#H !> %Φ HP HΦ".
+    iIntros "H %Φ HP HΦ".
     iDestruct (atomic_update_mask_weaken _ (⊤ ∖ E1) with "HΦ") as "HΦ"; first solve_ndisj.
     iSteps.
   Qed.
 
-  #[global] Instance frame_atomic_triple R e E P α β Ψ1 Ψ2 f :
-    (∀ x y, Frame true R (Ψ1 x y) (Ψ2 x y)) →
-    Frame true R (atomic_triple e E P α β (λ.. x y, Ψ1 x y) f) (atomic_triple e E P α β (λ.. x y, Ψ2 x y) f).
+  #[global] Instance frame_atomic_triple p R e E P α β Ψ1 Ψ2 f :
+    (∀ x y z, Frame p R (Ψ1 x y z) (Ψ2 x y z)) →
+    Frame p R (atomic_triple e E P α β (λ.. x y, Ψ1 x y) f) (atomic_triple e E P α β (λ.. x y, Ψ2 x y) f).
   Proof.
-    rewrite /Frame.
-    iIntros "/= %HΨ (#HR & H)".
-    iApply (atomic_triple_wand with "H"). iIntros "!> %x %y HΨ2". rewrite !tele_app_bind.
+    iIntros "/= %HΨ (HR & H)".
+    iApply (atomic_triple_wand with "H"). iIntros "%x %y %z HΨ2". rewrite !tele_app_bind.
     iApply HΨ.
     iSteps.
   Qed.
 End atomic_triple.
 
-Notation "'<<<' P | ∀∀ x1 .. xn , α '>>>' e @ E '<<<' ∃∃ y1 .. yn , β | 'RET' v ; Q '>>>'" := (
+Notation "'<<<' P | ∀∀ x1 .. xn , α '>>>' e @ E '<<<' ∃∃ y1 .. yn , β | z1 .. zn , 'RET' v ; Q '>>>'" := (
   atomic_triple
-    (TA := TeleS (λ x1, .. (TeleS (λ xn, TeleO)) .. ))
-    (TB := TeleS (λ y1, .. (TeleS (λ yn, TeleO)) .. ))
+    (TA := TeleS (λ x1, .. (TeleS (λ xn, TeleO)) ..))
+    (TB := TeleS (λ y1, .. (TeleS (λ yn, TeleO)) ..))
+    (TP := TeleS (λ z1, .. (TeleS (λ zn, TeleO)) ..))
     e%E
     E
     P%I
     (tele_app $ λ x1, .. (λ xn, α%I) ..)
-    (tele_app $ λ x1, .. (λ xn, tele_app (λ y1, .. (λ yn, β%I) .. )) .. )
-    (tele_app $ λ x1, .. (λ xn, tele_app (λ y1, .. (λ yn, Q%I) .. )) .. )
-    (tele_app $ λ x1, .. (λ xn, tele_app (λ y1, .. (λ yn, v%V) .. )) .. )
+    (tele_app $ λ x1, .. (λ xn, tele_app $ λ y1, .. (λ yn, β%I) ..) ..)
+    (tele_app $ λ x1, .. (λ xn, tele_app $ λ y1, .. (λ yn, tele_app $ λ z1, .. (λ zn, Q%I) ..) ..) ..)
+    (tele_app $ λ x1, .. (λ xn, tele_app $ λ y1, .. (λ yn, tele_app $ λ z1, .. (λ zn, v%V) ..) ..) ..)
+)(at level 20,
+  P, α, e, E, β, v, Q at level 200,
+  x1 binder,
+  xn binder,
+  y1 binder,
+  yn binder,
+  z1 binder,
+  zn binder,
+  format "'[hv' <<<  '/  ' '[' P ']'  '/' |  ∀∀  x1  ..  xn ,  '/  ' '[' α ']'  '/' >>>  '/  ' '[hv' e  '/' @  E ']'  '/' <<<  '/  ' ∃∃  y1  ..  yn ,  '/  ' '[' β ']'  '/' |  z1  ..  zn ,  '/  ' RET  v ;  '/  ' '[' Q ']'  '/' >>> ']'"
+) : bi_scope.
+Notation "'<<<' P | ∀∀ x1 .. xn , α '>>>' e @ E '<<<' ∃∃ y1 .. yn , β | 'RET' v ; Q '>>>'" := (
+  atomic_triple
+    (TA := TeleS (λ x1, .. (TeleS (λ xn, TeleO)) ..))
+    (TB := TeleS (λ y1, .. (TeleS (λ yn, TeleO)) ..))
+    (TP := TeleO)
+    e%E
+    E
+    P%I
+    (tele_app $ λ x1, .. (λ xn, α%I) ..)
+    (tele_app $ λ x1, .. (λ xn, tele_app $ λ y1, .. (λ yn, β%I) ..) ..)
+    (tele_app $ λ x1, .. (λ xn, tele_app $ λ y1, .. (λ yn, tele_app Q%I) ..) ..)
+    (tele_app $ λ x1, .. (λ xn, tele_app $ λ y1, .. (λ yn, tele_app v%V) ..) ..)
 )(at level 20,
   P, α, e, E, β, v, Q at level 200,
   x1 binder,
@@ -513,116 +307,151 @@ Notation "'<<<' P | ∀∀ x1 .. xn , α '>>>' e @ E '<<<' ∃∃ y1 .. yn , β 
   yn binder,
   format "'[hv' <<<  '/  ' '[' P ']'  '/' |  ∀∀  x1  ..  xn ,  '/  ' '[' α ']'  '/' >>>  '/  ' '[hv' e  '/' @  E ']'  '/' <<<  '/  ' ∃∃  y1  ..  yn ,  '/  ' '[' β ']'  '/' |  RET  v ;  '/  ' '[' Q ']'  '/' >>> ']'"
 ) : bi_scope.
-Notation "'<<<' P | α '>>>' e @ E '<<<' ∃∃ y1 .. yn , β | 'RET' v ; Q '>>>'" := (
+Notation "'<<<' P | ∀∀ x1 .. xn , α '>>>' e @ E '<<<' β | z1 .. zn , 'RET' v ; Q '>>>'" := (
   atomic_triple
-    (TA := TeleO)
-    (TB := TeleS (λ y1, .. (TeleS (λ yn, TeleO)) .. ))
-    e%E
-    E
-    P%I
-    (tele_app α%I)
-    (tele_app $ tele_app (λ y1, .. (λ yn, β%I) .. ))
-    (tele_app $ tele_app (λ y1, .. (λ yn, Q%I) .. ))
-    (tele_app $ tele_app (λ y1, .. (λ yn, v%V) .. ))
-)(at level 20,
-  P, α, e, E, β, v, Q at level 200,
-  y1 binder,
-  yn binder,
-  format "'[hv' <<<  '/  ' '[' P ']'  '/' |  '[' α ']'  '/' >>>  '/  ' '[hv' e  '/' @  E ']'  '/' <<<  '/  ' ∃∃  y1  ..  yn ,  '/  ' '[' β ']'  '/' |  RET  v ;  '/  ' '[' Q ']'  '/' >>> ']'"
-) : bi_scope.
-Notation "'<<<' P | ∀∀ x1 .. xn , α '>>>' e @ E '<<<' β | 'RET' v ; Q '>>>'" := (
-  atomic_triple
-    (TA := TeleS (λ x1, .. (TeleS (λ xn, TeleO)) .. ))
+    (TA := TeleS (λ x1, .. (TeleS (λ xn, TeleO)) ..))
     (TB := TeleO)
+    (TP := TeleS (λ z1, .. (TeleS (λ zn, TeleO)) ..))
     e%E
     E
     P%I
     (tele_app $ λ x1, .. (λ xn, α%I) ..)
-    (tele_app $ λ x1, .. (λ xn, tele_app β%I) .. )
-    (tele_app $ λ x1, .. (λ xn, tele_app Q%I) .. )
-    (tele_app $ λ x1, .. (λ xn, tele_app v%V) .. )
+    (tele_app $ λ x1, .. (λ xn, tele_app β%I) ..)
+    (tele_app $ λ x1, .. (λ xn, tele_app $ tele_app $ λ z1, .. (λ zn, Q%I) ..) ..)
+    (tele_app $ λ x1, .. (λ xn, tele_app $ tele_app $ λ z1, .. (λ zn, v%V) ..) ..)
+)(at level 20,
+  P, α, e, E, β, v, Q at level 200,
+  x1 binder,
+  xn binder,
+  z1 binder,
+  zn binder,
+  format "'[hv' <<<  '/  ' '[' P ']'  '/' |  ∀∀  x1  ..  xn ,  '/  ' '[' α ']'  '/' >>>  '/  ' '[hv' e  '/' @  E ']'  '/' <<<  '/  ' '[' β ']'  '/' |  z1  ..  zn ,  '/  ' RET  v ;  '/  ' '[' Q ']'  '/' >>> ']'"
+) : bi_scope.
+Notation "'<<<' P | ∀∀ x1 .. xn , α '>>>' e @ E '<<<' β | 'RET' v ; Q '>>>'" := (
+  atomic_triple
+    (TA := TeleS (λ x1, .. (TeleS (λ xn, TeleO)) ..))
+    (TB := TeleO)
+    (TP := TeleO)
+    e%E
+    E
+    P%I
+    (tele_app $ λ x1, .. (λ xn, α%I) ..)
+    (tele_app $ λ x1, .. (λ xn, tele_app β%I) ..)
+    (tele_app $ λ x1, .. (λ xn, tele_app $ tele_app Q%I) ..)
+    (tele_app $ λ x1, .. (λ xn, tele_app $ tele_app v%V) ..)
 )(at level 20,
   P, α, e, E, β, v, Q at level 200,
   x1 binder,
   xn binder,
   format "'[hv' <<<  '/  ' '[' P ']'  '/' |  ∀∀  x1  ..  xn ,  '/  ' '[' α ']'  '/' >>>  '/  ' '[hv' e  '/' @  E ']'  '/' <<<  '/  ' '[' β ']'  '/' |  RET  v ;  '/  ' '[' Q ']'  '/' >>> ']'"
 ) : bi_scope.
-Notation "'<<<' P | α '>>>' e @ E '<<<' β | 'RET' v ; Q '>>>'" := (
+Notation "'<<<' P | α '>>>' e @ E '<<<' ∃∃ y1 .. yn , β | z1 .. zn , 'RET' v ; Q '>>>'" := (
+  atomic_triple
+    (TA := TeleO)
+    (TB := TeleS (λ y1, .. (TeleS (λ yn, TeleO)) ..))
+    (TP := TeleS (λ z1, .. (TeleS (λ zn, TeleO)) ..))
+    e%E
+    E
+    P%I
+    (tele_app α%I)
+    (tele_app $ tele_app $ λ y1, .. (λ yn, β%I) ..)
+    (tele_app $ tele_app $ λ y1, .. (λ yn, tele_app $ λ z1, .. (λ zn, Q%I) ..) ..)
+    (tele_app $ tele_app $ λ y1, .. (λ yn, tele_app v%V) ..)
+)(at level 20,
+  P, α, e, E, β, v, Q at level 200,
+  y1 binder,
+  yn binder,
+  z1 binder,
+  zn binder,
+  format "'[hv' <<<  '/  ' '[' P ']'  '/' |  '[' α ']'  '/' >>>  '/  ' '[hv' e  '/' @  E ']'  '/' <<<  '/  ' ∃∃  y1  ..  yn ,  '/  ' '[' β ']'  '/' |  z1  ..  zn ,  '/  ' RET  v ;  '/  ' '[' Q ']'  '/' >>> ']'"
+) : bi_scope.
+Notation "'<<<' P | α '>>>' e @ E '<<<' ∃∃ y1 .. yn , β | 'RET' v ; Q '>>>'" := (
+  atomic_triple
+    (TA := TeleO)
+    (TB := TeleS (λ y1, .. (TeleS (λ yn, TeleO)) ..))
+    (TP := TeleO)
+    e%E
+    E
+    P%I
+    (tele_app α%I)
+    (tele_app $ tele_app $ λ y1, .. (λ yn, β%I) ..)
+    (tele_app $ tele_app $ λ y1, .. (λ yn, tele_app Q%I) ..)
+    (tele_app $ tele_app $ λ y1, .. (λ yn, tele_app v%V) ..)
+)(at level 20,
+  P, α, e, E, β, v, Q at level 200,
+  y1 binder,
+  yn binder,
+  format "'[hv' <<<  '/  ' '[' P ']'  '/' |  '[' α ']'  '/' >>>  '/  ' '[hv' e  '/' @  E ']'  '/' <<<  '/  ' ∃∃  y1  ..  yn ,  '/  ' '[' β ']'  '/' |  RET  v ;  '/  ' '[' Q ']'  '/' >>> ']'"
+) : bi_scope.
+Notation "'<<<' P | α '>>>' e @ E '<<<' β | z1 .. zn , 'RET' v ; Q '>>>'" := (
   atomic_triple
     (TA := TeleO)
     (TB := TeleO)
+    (TP := TeleS (λ z1, .. (TeleS (λ zn, TeleO)) ..))
     e%E
     E
     P%I
     (tele_app α%I)
     (tele_app $ tele_app β%I)
-    (tele_app $ tele_app Q%I)
-    (tele_app $ tele_app v%V)
+    (tele_app $ tele_app $ tele_app $ λ z1, .. (λ zn, Q%I) ..)
+    (tele_app $ tele_app $ tele_app $ λ z1, .. (λ zn, v%V) ..)
+)(at level 20,
+  P, α, e, E, β, v, Q at level 200,
+  z1 binder,
+  zn binder,
+  format "'[hv' <<<  '/  ' '[' P ']'  '/' |  '[' α ']'  '/' >>>  '/  ' '[hv' e  '/' @  E ']'  '/' <<<  '/  ' '[' β ']'  '/' |  z1  ..  zn ,  '/  ' RET  v ;  '/  ' '[' Q ']'  '/' >>> ']'"
+) : bi_scope.
+Notation "'<<<' P | α '>>>' e @ E '<<<' β | 'RET' v ; Q '>>>'" := (
+  atomic_triple
+    (TA := TeleO)
+    (TB := TeleO)
+    (TP := TeleO)
+    e%E
+    E
+    P%I
+    (tele_app α%I)
+    (tele_app $ tele_app β%I)
+    (tele_app $ tele_app $ tele_app Q%I)
+    (tele_app $ tele_app $ tele_app v%V)
 )(at level 20,
   P, α, e, E, β, v, Q at level 200,
   format "'[hv' <<<  '/  ' '[' P ']'  '/' |  '[' α ']'  '/' >>>  '/  ' '[hv' e  '/' @  E ']'  '/' <<<  '/  ' '[' β ']'  '/' |  RET  v ;  '/  ' '[' Q ']'  '/' >>> ']'"
 ) : bi_scope.
 
-Notation "'<<<' P | ∀∀ x1 .. xn , α '>>>' e @ E '<<<' ∃∃ y1 .. yn , β | 'RET' v ; Q '>>>'" := (
-  ⊢ atomic_triple
-    (TA := TeleS (λ x1, .. (TeleS (λ xn, TeleO)) .. ))
-    (TB := TeleS (λ y1, .. (TeleS (λ yn, TeleO)) .. ))
-    e%E
-    E
-    P%I
-    (tele_app $ λ x1, .. (λ xn, α%I) ..)
-    (tele_app $ λ x1, .. (λ xn, tele_app (λ y1, .. (λ yn, β%I) .. )) .. )
-    (tele_app $ λ x1, .. (λ xn, tele_app (λ y1, .. (λ yn, Q%I) .. )) .. )
-    (tele_app $ λ x1, .. (λ xn, tele_app (λ y1, .. (λ yn, v%V) .. )) .. )
-) : stdpp_scope.
-Notation "'<<<' P | α '>>>' e @ E '<<<' ∃∃ y1 .. yn , β | 'RET' v ; Q '>>>'" := (
-  ⊢ atomic_triple
-    (TA := TeleO)
-    (TB := TeleS (λ y1, .. (TeleS (λ yn, TeleO)) .. ))
-    e%E
-    E
-    P%I
-    (tele_app α%I)
-    (tele_app $ tele_app (λ y1, .. (λ yn, β%I) .. ))
-    (tele_app $ tele_app (λ y1, .. (λ yn, Q%I) .. ))
-    (tele_app $ tele_app (λ y1, .. (λ yn, v%V) .. ))
-) : stdpp_scope.
-Notation "'<<<' P | ∀∀ x1 .. xn , α '>>>' e @ E '<<<' β | 'RET' v ; Q '>>>'" := (
-  ⊢ atomic_triple
-    (TA := TeleS (λ x1, .. (TeleS (λ xn, TeleO)) .. ))
-    (TB := TeleO)
-    e%E
-    E
-    P%I
-    (tele_app $ λ x1, .. (λ xn, α%I) ..)
-    (tele_app $ λ x1, .. (λ xn, tele_app β%I) .. )
-    (tele_app $ λ x1, .. (λ xn, tele_app Q%I) .. )
-    (tele_app $ λ x1, .. (λ xn, tele_app v%V) .. )
-) : stdpp_scope.
-Notation "'<<<' P | α '>>>' e @ E '<<<' β | 'RET' v ; Q '>>>'" := (
-  ⊢ atomic_triple
-    (TA := TeleO)
-    (TB := TeleO)
-    e%E
-    E
-    P%I
-    (tele_app α%I)
-    (tele_app $ tele_app β%I)
-    (tele_app $ tele_app Q%I)
-    (tele_app $ tele_app v%V)
-) : stdpp_scope.
-
-Notation "'<<<' P | ∀∀ x1 .. xn , α '>>>' e '<<<' ∃∃ y1 .. yn , β | 'RET' v ; Q '>>>'" := (
+Notation "'<<<' P | ∀∀ x1 .. xn , α '>>>' e '<<<' ∃∃ y1 .. yn , β | z1 .. zn , 'RET' v ; Q '>>>'" := (
   atomic_triple
-    (TA := TeleS (λ x1, .. (TeleS (λ xn, TeleO)) .. ))
-    (TB := TeleS (λ y1, .. (TeleS (λ yn, TeleO)) .. ))
+    (TA := TeleS (λ x1, .. (TeleS (λ xn, TeleO)) ..))
+    (TB := TeleS (λ y1, .. (TeleS (λ yn, TeleO)) ..))
+    (TP := TeleS (λ z1, .. (TeleS (λ zn, TeleO)) ..))
     e%E
     ∅
     P%I
     (tele_app $ λ x1, .. (λ xn, α%I) ..)
-    (tele_app $ λ x1, .. (λ xn, tele_app (λ y1, .. (λ yn, β%I) .. )) .. )
-    (tele_app $ λ x1, .. (λ xn, tele_app (λ y1, .. (λ yn, Q%I) .. )) .. )
-    (tele_app $ λ x1, .. (λ xn, tele_app (λ y1, .. (λ yn, v%V) .. )) .. )
+    (tele_app $ λ x1, .. (λ xn, tele_app $ λ y1, .. (λ yn, β%I) ..) ..)
+    (tele_app $ λ x1, .. (λ xn, tele_app $ λ y1, .. (λ yn, tele_app $ λ z1, .. (λ zn, Q%I) ..) ..) ..)
+    (tele_app $ λ x1, .. (λ xn, tele_app $ λ y1, .. (λ yn, tele_app $ λ z1, .. (λ zn, v%V) ..) ..) ..)
+)(at level 20,
+  P, α, e, β, v, Q at level 200,
+  x1 binder,
+  xn binder,
+  y1 binder,
+  yn binder,
+  z1 binder,
+  zn binder,
+  format "'[hv' <<<  '/  ' '[' P ']'  '/' |  ∀∀  x1  ..  xn ,  '/  ' '[' α ']'  '/' >>>  '/  ' '[' e ']'  '/' <<<  '/  ' ∃∃  y1  ..  yn ,  '/  ' '[' β ']'  '/' |  z1  ..  zn ,  '/  ' RET  v ;  '/  ' '[' Q ']'  '/' >>> ']'"
+) : bi_scope.
+Notation "'<<<' P | ∀∀ x1 .. xn , α '>>>' e '<<<' ∃∃ y1 .. yn , β | 'RET' v ; Q '>>>'" := (
+  atomic_triple
+    (TA := TeleS (λ x1, .. (TeleS (λ xn, TeleO)) ..))
+    (TB := TeleS (λ y1, .. (TeleS (λ yn, TeleO)) ..))
+    (TP := TeleO)
+    e%E
+    ∅
+    P%I
+    (tele_app $ λ x1, .. (λ xn, α%I) ..)
+    (tele_app $ λ x1, .. (λ xn, tele_app $ λ y1, .. (λ yn, β%I) ..) ..)
+    (tele_app $ λ x1, .. (λ xn, tele_app $ λ y1, .. (λ yn, tele_app Q%I) ..) ..)
+    (tele_app $ λ x1, .. (λ xn, tele_app $ λ y1, .. (λ yn, tele_app v%V) ..) ..)
 )(at level 20,
   P, α, e, β, v, Q at level 200,
   x1 binder,
@@ -631,101 +460,323 @@ Notation "'<<<' P | ∀∀ x1 .. xn , α '>>>' e '<<<' ∃∃ y1 .. yn , β | 'R
   yn binder,
   format "'[hv' <<<  '/  ' '[' P ']'  '/' |  ∀∀  x1  ..  xn ,  '/  ' '[' α ']'  '/' >>>  '/  ' '[' e ']'  '/' <<<  '/  ' ∃∃  y1  ..  yn ,  '/  ' '[' β ']'  '/' |  RET  v ;  '/  ' '[' Q ']'  '/' >>> ']'"
 ) : bi_scope.
-Notation "'<<<' P | α '>>>' e '<<<' ∃∃ y1 .. yn , β | 'RET' v ; Q '>>>'" := (
+Notation "'<<<' P | ∀∀ x1 .. xn , α '>>>' e '<<<' β | z1 .. zn , 'RET' v ; Q '>>>'" := (
   atomic_triple
-    (TA := TeleO)
-    (TB := TeleS (λ y1, .. (TeleS (λ yn, TeleO)) .. ))
-    e%E
-    ∅
-    P%I
-    (tele_app α%I)
-    (tele_app $ tele_app (λ y1, .. (λ yn, β%I) .. ))
-    (tele_app $ tele_app (λ y1, .. (λ yn, Q%I) .. ))
-    (tele_app $ tele_app (λ y1, .. (λ yn, v%V) .. ))
-)(at level 20,
-  P, α, e, β, v, Q at level 200,
-  y1 binder,
-  yn binder,
-  format "'[hv' <<<  '/  ' '[' P ']'  '/' |  '[' α ']'  '/' >>>  '/  ' '[' e ']'  '/' <<<  '/  ' ∃∃  y1  ..  yn ,  '/  ' '[' β ']'  '/' |  RET  v ;  '/  ' '[' Q ']'  '/' >>> ']'"
-) : bi_scope.
-Notation "'<<<' P | ∀∀ x1 .. xn , α '>>>' e '<<<' β | 'RET' v ; Q '>>>'" := (
-  atomic_triple
-    (TA := TeleS (λ x1, .. (TeleS (λ xn, TeleO)) .. ))
+    (TA := TeleS (λ x1, .. (TeleS (λ xn, TeleO)) ..))
     (TB := TeleO)
+    (TP := TeleS (λ z1, .. (TeleS (λ zn, TeleO)) ..))
     e%E
     ∅
     P%I
     (tele_app $ λ x1, .. (λ xn, α%I) ..)
-    (tele_app $ λ x1, .. (λ xn, tele_app β%I) .. )
-    (tele_app $ λ x1, .. (λ xn, tele_app Q%I) .. )
-    (tele_app $ λ x1, .. (λ xn, tele_app v%V) .. )
+    (tele_app $ λ x1, .. (λ xn, tele_app β%I) ..)
+    (tele_app $ λ x1, .. (λ xn, tele_app $ tele_app $ λ z1, .. (λ zn, Q%I) ..) ..)
+    (tele_app $ λ x1, .. (λ xn, tele_app $ tele_app $ λ z1, .. (λ zn, v%V) ..) ..)
+)(at level 20,
+  P, α, e, β, v, Q at level 200,
+  x1 binder,
+  xn binder,
+  z1 binder,
+  zn binder,
+  format "'[hv' <<<  '/  ' '[' P ']'  '/' |  ∀∀  x1  ..  xn ,  '/  ' '[' α ']'  '/' >>>  '/  ' '[' e ']'  '/' <<<  '/  ' '[' β ']'  '/' |  z1  ..  zn ,  '/  ' RET  v ;  '/  ' '[' Q ']'  '/' >>> ']'"
+) : bi_scope.
+Notation "'<<<' P | ∀∀ x1 .. xn , α '>>>' e '<<<' β | 'RET' v ; Q '>>>'" := (
+  atomic_triple
+    (TA := TeleS (λ x1, .. (TeleS (λ xn, TeleO)) ..))
+    (TB := TeleO)
+    (TP := TeleO)
+    e%E
+    ∅
+    P%I
+    (tele_app $ λ x1, .. (λ xn, α%I) ..)
+    (tele_app $ λ x1, .. (λ xn, tele_app β%I) ..)
+    (tele_app $ λ x1, .. (λ xn, tele_app $ tele_app Q%I) ..)
+    (tele_app $ λ x1, .. (λ xn, tele_app $ tele_app v%V) ..)
 )(at level 20,
   P, α, e, β, v, Q at level 200,
   x1 binder,
   xn binder,
   format "'[hv' <<<  '/  ' '[' P ']'  '/' |  ∀∀  x1  ..  xn ,  '/  ' '[' α ']'  '/' >>>  '/  ' '[' e ']'  '/' <<<  '/  ' '[' β ']'  '/' |  RET  v ;  '/  ' '[' Q ']'  '/' >>> ']'"
 ) : bi_scope.
-Notation "'<<<' P | α '>>>' e '<<<' β | 'RET' v ; Q '>>>'" := (
+Notation "'<<<' P | α '>>>' e '<<<' ∃∃ y1 .. yn , β | z1 .. zn , 'RET' v ; Q '>>>'" := (
+  atomic_triple
+    (TA := TeleO)
+    (TB := TeleS (λ y1, .. (TeleS (λ yn, TeleO)) ..))
+    (TP := TeleS (λ z1, .. (TeleS (λ zn, TeleO)) ..))
+    e%E
+    ∅
+    P%I
+    (tele_app α%I)
+    (tele_app $ tele_app $ λ y1, .. (λ yn, β%I) ..)
+    (tele_app $ tele_app $ λ y1, .. (λ yn, tele_app $ λ z1, .. (λ zn, Q%I) ..) ..)
+    (tele_app $ tele_app $ λ y1, .. (λ yn, tele_app v%V) ..)
+)(at level 20,
+  P, α, e, β, v, Q at level 200,
+  y1 binder,
+  yn binder,
+  z1 binder,
+  zn binder,
+  format "'[hv' <<<  '/  ' '[' P ']'  '/' |  '[' α ']'  '/' >>>  '/  ' '[' e ']'  '/' <<<  '/  ' ∃∃  y1  ..  yn ,  '/  ' '[' β ']'  '/' |  z1  ..  zn ,  '/  ' RET  v ;  '/  ' '[' Q ']'  '/' >>> ']'"
+) : bi_scope.
+Notation "'<<<' P | α '>>>' e '<<<' ∃∃ y1 .. yn , β | 'RET' v ; Q '>>>'" := (
+  atomic_triple
+    (TA := TeleO)
+    (TB := TeleS (λ y1, .. (TeleS (λ yn, TeleO)) ..))
+    (TP := TeleO)
+    e%E
+    ∅
+    P%I
+    (tele_app α%I)
+    (tele_app $ tele_app $ λ y1, .. (λ yn, β%I) ..)
+    (tele_app $ tele_app $ λ y1, .. (λ yn, tele_app Q%I) ..)
+    (tele_app $ tele_app $ λ y1, .. (λ yn, tele_app v%V) ..)
+)(at level 20,
+  P, α, e, β, v, Q at level 200,
+  y1 binder,
+  yn binder,
+  format "'[hv' <<<  '/  ' '[' P ']'  '/' |  '[' α ']'  '/' >>>  '/  ' '[' e ']'  '/' <<<  '/  ' ∃∃  y1  ..  yn ,  '/  ' '[' β ']'  '/' |  RET  v ;  '/  ' '[' Q ']'  '/' >>> ']'"
+) : bi_scope.
+Notation "'<<<' P | α '>>>' e '<<<' β | z1 .. zn , 'RET' v ; Q '>>>'" := (
   atomic_triple
     (TA := TeleO)
     (TB := TeleO)
+    (TP := TeleS (λ z1, .. (TeleS (λ zn, TeleO)) ..))
     e%E
     ∅
     P%I
     (tele_app α%I)
     (tele_app $ tele_app β%I)
-    (tele_app $ tele_app Q%I)
-    (tele_app $ tele_app v%V)
+    (tele_app $ tele_app $ tele_app $ λ z1, .. (λ zn, Q%I) ..)
+    (tele_app $ tele_app $ tele_app $ λ z1, .. (λ zn, v%V) ..)
+)(at level 20,
+  P, α, e, β, v, Q at level 200,
+  z1 binder,
+  zn binder,
+  format "'[hv' <<<  '/  ' '[' P ']'  '/' |  '[' α ']'  '/' >>>  '/  ' '[' e ']'  '/' <<<  '/  ' '[' β ']'  '/' |  z1  ..  zn ,  '/  ' RET  v ;  '/  ' '[' Q ']'  '/' >>> ']'"
+) : bi_scope.
+Notation "'<<<' P | α '>>>' e '<<<' β | 'RET' v ; Q '>>>'" := (
+  atomic_triple
+    (TA := TeleO)
+    (TB := TeleO)
+    (TP := TeleO)
+    e%E
+    ∅
+    P%I
+    (tele_app α%I)
+    (tele_app $ tele_app β%I)
+    (tele_app $ tele_app $ tele_app Q%I)
+    (tele_app $ tele_app $ tele_app v%V)
 )(at level 20,
   P, α, e, β, v, Q at level 200,
   format "'[hv' <<<  '/  ' '[' P ']'  '/' |  '[' α ']'  '/' >>>  '/  ' '[' e ']'  '/' <<<  '/  ' '[' β ']'  '/' |  RET  v ;  '/  ' '[' Q ']'  '/' >>> ']'"
 ) : bi_scope.
 
-Notation "'<<<' P | ∀∀ x1 .. xn , α '>>>' e '<<<' ∃∃ y1 .. yn , β | 'RET' v ; Q '>>>'" := (
+Notation "'<<<' P | ∀∀ x1 .. xn , α '>>>' e @ E '<<<' ∃∃ y1 .. yn , β | z1 .. zn , 'RET' v ; Q '>>>'" := (
   ⊢ atomic_triple
-    (TA := TeleS (λ x1, .. (TeleS (λ xn, TeleO)) .. ))
-    (TB := TeleS (λ y1, .. (TeleS (λ yn, TeleO)) .. ))
+    (TA := TeleS (λ x1, .. (TeleS (λ xn, TeleO)) ..))
+    (TB := TeleS (λ y1, .. (TeleS (λ yn, TeleO)) ..))
+    (TP := TeleS (λ z1, .. (TeleS (λ zn, TeleO)) ..))
+    e%E
+    E
+    P%I
+    (tele_app $ λ x1, .. (λ xn, α%I) ..)
+    (tele_app $ λ x1, .. (λ xn, tele_app $ λ y1, .. (λ yn, β%I) ..) ..)
+    (tele_app $ λ x1, .. (λ xn, tele_app $ λ y1, .. (λ yn, tele_app $ λ z1, .. (λ zn, Q%I) ..) ..) ..)
+    (tele_app $ λ x1, .. (λ xn, tele_app $ λ y1, .. (λ yn, tele_app $ λ z1, .. (λ zn, v%V) ..) ..) ..)
+) : stdpp_scope.
+Notation "'<<<' P | ∀∀ x1 .. xn , α '>>>' e @ E '<<<' ∃∃ y1 .. yn , β | 'RET' v ; Q '>>>'" := (
+  ⊢ atomic_triple
+    (TA := TeleS (λ x1, .. (TeleS (λ xn, TeleO)) ..))
+    (TB := TeleS (λ y1, .. (TeleS (λ yn, TeleO)) ..))
+    (TP := TeleO)
+    e%E
+    E
+    P%I
+    (tele_app $ λ x1, .. (λ xn, α%I) ..)
+    (tele_app $ λ x1, .. (λ xn, tele_app $ λ y1, .. (λ yn, β%I) ..) ..)
+    (tele_app $ λ x1, .. (λ xn, tele_app $ λ y1, .. (λ yn, tele_app Q%I) ..) ..)
+    (tele_app $ λ x1, .. (λ xn, tele_app $ λ y1, .. (λ yn, tele_app v%V) ..) ..)
+) : stdpp_scope.
+Notation "'<<<' P | ∀∀ x1 .. xn , α '>>>' e @ E '<<<' β | z1 .. zn , 'RET' v ; Q '>>>'" := (
+  ⊢ atomic_triple
+    (TA := TeleS (λ x1, .. (TeleS (λ xn, TeleO)) ..))
+    (TB := TeleO)
+    (TP := TeleS (λ z1, .. (TeleS (λ zn, TeleO)) ..))
+    e%E
+    E
+    P%I
+    (tele_app $ λ x1, .. (λ xn, α%I) ..)
+    (tele_app $ λ x1, .. (λ xn, tele_app β%I) ..)
+    (tele_app $ λ x1, .. (λ xn, tele_app $ tele_app $ λ z1, .. (λ zn, Q%I) ..) ..)
+    (tele_app $ λ x1, .. (λ xn, tele_app $ tele_app $ λ z1, .. (λ zn, v%V) ..) ..)
+) : stdpp_scope.
+Notation "'<<<' P | ∀∀ x1 .. xn , α '>>>' e @ E '<<<' β | 'RET' v ; Q '>>>'" := (
+  ⊢ atomic_triple
+    (TA := TeleS (λ x1, .. (TeleS (λ xn, TeleO)) ..))
+    (TB := TeleO)
+    (TP := TeleO)
+    e%E
+    E
+    P%I
+    (tele_app $ λ x1, .. (λ xn, α%I) ..)
+    (tele_app $ λ x1, .. (λ xn, tele_app β%I) ..)
+    (tele_app $ λ x1, .. (λ xn, tele_app $ tele_app Q%I) ..)
+    (tele_app $ λ x1, .. (λ xn, tele_app $ tele_app v%V) ..)
+) : stdpp_scope.
+Notation "'<<<' P | α '>>>' e @ E '<<<' ∃∃ y1 .. yn , β | z1 .. zn , 'RET' v ; Q '>>>'" := (
+  ⊢ atomic_triple
+    (TA := TeleO)
+    (TB := TeleS (λ y1, .. (TeleS (λ yn, TeleO)) ..))
+    (TP := TeleS (λ z1, .. (TeleS (λ zn, TeleO)) ..))
+    e%E
+    E
+    P%I
+    (tele_app α%I)
+    (tele_app $ tele_app $ λ y1, .. (λ yn, β%I) ..)
+    (tele_app $ tele_app $ λ y1, .. (λ yn, tele_app $ λ z1, .. (λ zn, Q%I) ..) ..)
+    (tele_app $ tele_app $ λ y1, .. (λ yn, tele_app v%V) ..)
+) : stdpp_scope.
+Notation "'<<<' P | α '>>>' e @ E '<<<' ∃∃ y1 .. yn , β | 'RET' v ; Q '>>>'" := (
+  ⊢ atomic_triple
+    (TA := TeleO)
+    (TB := TeleS (λ y1, .. (TeleS (λ yn, TeleO)) ..))
+    (TP := TeleO)
+    e%E
+    E
+    P%I
+    (tele_app α%I)
+    (tele_app $ tele_app $ λ y1, .. (λ yn, β%I) ..)
+    (tele_app $ tele_app $ λ y1, .. (λ yn, tele_app Q%I) ..)
+    (tele_app $ tele_app $ λ y1, .. (λ yn, tele_app v%V) ..)
+) : stdpp_scope.
+Notation "'<<<' P | α '>>>' e @ E '<<<' β | z1 .. zn , 'RET' v ; Q '>>>'" := (
+  ⊢ atomic_triple
+    (TA := TeleO)
+    (TB := TeleO)
+    (TP := TeleS (λ z1, .. (TeleS (λ zn, TeleO)) ..))
+    e%E
+    E
+    P%I
+    (tele_app α%I)
+    (tele_app $ tele_app β%I)
+    (tele_app $ tele_app $ tele_app $ λ z1, .. (λ zn, Q%I) ..)
+    (tele_app $ tele_app $ tele_app $ λ z1, .. (λ zn, v%V) ..)
+) : stdpp_scope.
+Notation "'<<<' P | α '>>>' e @ E '<<<' β | 'RET' v ; Q '>>>'" := (
+  ⊢ atomic_triple
+    (TA := TeleO)
+    (TB := TeleO)
+    (TP := TeleO)
+    e%E
+    E
+    P%I
+    (tele_app α%I)
+    (tele_app $ tele_app β%I)
+    (tele_app $ tele_app $ tele_app Q%I)
+    (tele_app $ tele_app $ tele_app v%V)
+) : stdpp_scope.
+
+Notation "'<<<' P | ∀∀ x1 .. xn , α '>>>' e '<<<' ∃∃ y1 .. yn , β | z1 .. zn , 'RET' v ; Q '>>>'" := (
+  ⊢ atomic_triple
+    (TA := TeleS (λ x1, .. (TeleS (λ xn, TeleO)) ..))
+    (TB := TeleS (λ y1, .. (TeleS (λ yn, TeleO)) ..))
+    (TP := TeleS (λ z1, .. (TeleS (λ zn, TeleO)) ..))
     e%E
     ∅
     P%I
     (tele_app $ λ x1, .. (λ xn, α%I) ..)
-    (tele_app $ λ x1, .. (λ xn, tele_app (λ y1, .. (λ yn, β%I) .. )) .. )
-    (tele_app $ λ x1, .. (λ xn, tele_app (λ y1, .. (λ yn, Q%I) .. )) .. )
-    (tele_app $ λ x1, .. (λ xn, tele_app (λ y1, .. (λ yn, v%V) .. )) .. )
+    (tele_app $ λ x1, .. (λ xn, tele_app $ λ y1, .. (λ yn, β%I) ..) ..)
+    (tele_app $ λ x1, .. (λ xn, tele_app $ λ y1, .. (λ yn, tele_app $ λ z1, .. (λ zn, Q%I) ..) ..) ..)
+    (tele_app $ λ x1, .. (λ xn, tele_app $ λ y1, .. (λ yn, tele_app $ λ z1, .. (λ zn, v%V) ..) ..) ..)
 ) : stdpp_scope.
-Notation "'<<<' P | α '>>>' e '<<<' ∃∃ y1 .. yn , β | 'RET' v ; Q '>>>'" := (
+Notation "'<<<' P | ∀∀ x1 .. xn , α '>>>' e '<<<' ∃∃ y1 .. yn , β | 'RET' v ; Q '>>>'" := (
+  ⊢ atomic_triple
+    (TA := TeleS (λ x1, .. (TeleS (λ xn, TeleO)) ..))
+    (TB := TeleS (λ y1, .. (TeleS (λ yn, TeleO)) ..))
+    (TP := TeleO)
+    e%E
+    ∅
+    P%I
+    (tele_app $ λ x1, .. (λ xn, α%I) ..)
+    (tele_app $ λ x1, .. (λ xn, tele_app $ λ y1, .. (λ yn, β%I) ..) ..)
+    (tele_app $ λ x1, .. (λ xn, tele_app $ λ y1, .. (λ yn, tele_app Q%I) ..) ..)
+    (tele_app $ λ x1, .. (λ xn, tele_app $ λ y1, .. (λ yn, tele_app v%V) ..) ..)
+) : stdpp_scope.
+Notation "'<<<' P | ∀∀ x1 .. xn , α '>>>' e '<<<' β | z1 .. zn , 'RET' v ; Q '>>>'" := (
+  ⊢ atomic_triple
+    (TA := TeleS (λ x1, .. (TeleS (λ xn, TeleO)) ..))
+    (TB := TeleO)
+    (TP := TeleS (λ z1, .. (TeleS (λ zn, TeleO)) ..))
+    e%E
+    ∅
+    P%I
+    (tele_app $ λ x1, .. (λ xn, α%I) ..)
+    (tele_app $ λ x1, .. (λ xn, tele_app β%I) ..)
+    (tele_app $ λ x1, .. (λ xn, tele_app $ tele_app $ λ z1, .. (λ zn, Q%I) ..) ..)
+    (tele_app $ λ x1, .. (λ xn, tele_app $ tele_app $ λ z1, .. (λ zn, v%V) ..) ..)
+) : stdpp_scope.
+Notation "'<<<' P | ∀∀ x1 .. xn , α '>>>' e '<<<' β | 'RET' v ; Q '>>>'" := (
+  ⊢ atomic_triple
+    (TA := TeleS (λ x1, .. (TeleS (λ xn, TeleO)) ..))
+    (TB := TeleO)
+    (TP := TeleO)
+    e%E
+    ∅
+    P%I
+    (tele_app $ λ x1, .. (λ xn, α%I) ..)
+    (tele_app $ λ x1, .. (λ xn, tele_app β%I) ..)
+    (tele_app $ λ x1, .. (λ xn, tele_app $ tele_app Q%I) ..)
+    (tele_app $ λ x1, .. (λ xn, tele_app $ tele_app v%V) ..)
+) : stdpp_scope.
+Notation "'<<<' P | α '>>>' e '<<<' ∃∃ y1 .. yn , β | z1 .. zn , 'RET' v ; Q '>>>'" := (
   ⊢ atomic_triple
     (TA := TeleO)
-    (TB := TeleS (λ y1, .. (TeleS (λ yn, TeleO)) .. ))
+    (TB := TeleS (λ y1, .. (TeleS (λ yn, TeleO)) ..))
+    (TP := TeleS (λ z1, .. (TeleS (λ zn, TeleO)) ..))
     e%E
     ∅
     P%I
     (tele_app α%I)
-    (tele_app $ tele_app (λ y1, .. (λ yn, β%I) .. ))
-    (tele_app $ tele_app (λ y1, .. (λ yn, Q%I) .. ))
-    (tele_app $ tele_app (λ y1, .. (λ yn, v%V) .. ))
+    (tele_app $ tele_app $ λ y1, .. (λ yn, β%I) ..)
+    (tele_app $ tele_app $ λ y1, .. (λ yn, tele_app $ λ z1, .. (λ zn, Q%I) ..) ..)
+    (tele_app $ tele_app $ λ y1, .. (λ yn, tele_app v%V) ..)
 ) : stdpp_scope.
-Notation "'<<<' P | ∀∀ x1 .. xn , α '>>>' e '<<<' β | 'RET' v ; Q '>>>'" := (
+Notation "'<<<' P | α '>>>' e '<<<' ∃∃ y1 .. yn , β | 'RET' v ; Q '>>>'" := (
   ⊢ atomic_triple
-    (TA := TeleS (λ x1, .. (TeleS (λ xn, TeleO)) .. ))
-    (TB := TeleO)
+    (TA := TeleO)
+    (TB := TeleS (λ y1, .. (TeleS (λ yn, TeleO)) ..))
+    (TP := TeleO)
     e%E
     ∅
     P%I
-    (tele_app $ λ x1, .. (λ xn, α%I) ..)
-    (tele_app $ λ x1, .. (λ xn, tele_app β%I) .. )
-    (tele_app $ λ x1, .. (λ xn, tele_app Q%I) .. )
-    (tele_app $ λ x1, .. (λ xn, tele_app v%V) .. )
+    (tele_app α%I)
+    (tele_app $ tele_app $ λ y1, .. (λ yn, β%I) ..)
+    (tele_app $ tele_app $ λ y1, .. (λ yn, tele_app Q%I) ..)
+    (tele_app $ tele_app $ λ y1, .. (λ yn, tele_app v%V) ..)
 ) : stdpp_scope.
-Notation "'<<<' P | α '>>>' e '<<<' β | 'RET' v ; Q '>>>'" := (
+Notation "'<<<' P | α '>>>' e '<<<' β | z1 .. zn , 'RET' v ; Q '>>>'" := (
   ⊢ atomic_triple
     (TA := TeleO)
     (TB := TeleO)
+    (TP := TeleS (λ z1, .. (TeleS (λ zn, TeleO)) ..))
     e%E
     ∅
     P%I
     (tele_app α%I)
     (tele_app $ tele_app β%I)
-    (tele_app $ tele_app Q%I)
-    (tele_app $ tele_app v%V)
+    (tele_app $ tele_app $ tele_app $ λ z1, .. (λ zn, Q%I) ..)
+    (tele_app $ tele_app $ tele_app $ λ z1, .. (λ zn, v%V) ..)
+) : stdpp_scope.
+Notation "'<<<' P | α '>>>' e '<<<' β | 'RET' v ; Q '>>>'" := (
+  ⊢ atomic_triple
+    (TA := TeleO)
+    (TB := TeleO)
+    (TP := TeleO)
+    e%E
+    ∅
+    P%I
+    (tele_app α%I)
+    (tele_app $ tele_app β%I)
+    (tele_app $ tele_app $ tele_app Q%I)
+    (tele_app $ tele_app $ tele_app v%V)
 ) : stdpp_scope.
